lunarlander_sl/ext2/BigStepEx.thy
@@ -1,0 +1,446 @@
+theory BigStepEx
+  imports BigStepSimple
+begin
+
+subsection \<open>Examples\<close>
+
+definition A :: char where "A = CHR ''a''"
+definition B :: char where "B = CHR ''b''"
+definition X :: char where "X = CHR ''x''"
+definition Y :: char where "Y = CHR ''y''"
+definition Z :: char where "Z = CHR ''z''"
+definition ch1 :: cname where "ch1 = ''ch1''"
+definition ch2 :: cname where "ch2 = ''ch2''"
+
+subsubsection \<open>Example 1\<close>
+
+text \<open>
+   ch1?X; ch2!(X+1)
+|| ch1!3
+\<close>
+definition ex1a :: "'a proc" where
+  "ex1a = (Cm (ch1[?]X); Cm (ch2[!](\<lambda>s. val s X + 1)))"
+
+definition ex1b :: "'a proc" where
+  "ex1b = (Cm (ch1[!](\<lambda>_. 3)))"
+
+lemma ex1a_sp:
+  "spec_of ex1a
+           (wait_in_c ch1 (\<lambda>d v. wait_out_c ch2 (\<lambda>s. val s X + 1) (\<lambda>d. init) {{ X := (\<lambda>_. v) }}))"
+  unfolding ex1a_def
+  apply (rule Valid_receive_sp)
+  apply (rule spec_of_send)
+  done
+
+lemma ex1b_sp:
+  "spec_of ex1b
+           (wait_out_c ch1 (\<lambda>_. 3) (\<lambda>d. init))"
+  unfolding ex1b_def
+  apply (rule spec_of_send)
+  done
+
+lemma ex1:
+  "spec_of_global
+    (Parallel (Single ''a'' ex1a) {ch1}
+              (Single ''b'' ex1b))
+    (sync_gassn {ch1} {''a''} {''b''}
+      (single_assn ''a'' (wait_in_c ch1 (\<lambda>d v. wait_out_c ch2 (\<lambda>s. val s X + 1) (\<lambda>d. init) {{ X := (\<lambda>_. v) }} )))
+      (single_assn ''b'' (wait_out_c ch1 (\<lambda>_. 3) (\<lambda>d. init))))"
+  apply (rule spec_of_parallel)
+     apply (rule spec_of_single)
+     apply (rule ex1a_sp)
+    apply (rule spec_of_single)
+    apply (rule ex1b_sp)
+  by auto
+
+lemma ex1':
+  "spec_of_global
+    (Parallel (Single ''a'' ex1a) {ch1}
+              (Single ''b'' ex1b))
+    (sync_gassn {ch1} {''a''} {''b''}
+      (wait_in_cg ch1 (\<lambda>d v. wait_out_cg ch2 ''a'' (\<lambda>s. val s X + 1) (\<lambda>d. init_single {''a''}) {{X := (\<lambda>_. v)}}\<^sub>g at ''a''))
+      (wait_out_cg ch1 ''b'' (\<lambda>_. 3) (\<lambda>d. init_single {''b''})))"
+  apply (rule spec_of_global_post)
+   apply (rule ex1) apply clarify subgoal for s0
+    apply (auto simp: single_assn_wait_in single_assn_wait_out updg_subst2 single_assn_init)
+    by (rule entails_g_triv)
+  done
+
+lemma ex1'':
+  "spec_of_global
+    (Parallel (Single ''a'' ex1a) {ch1}
+              (Single ''b'' ex1b))
+    (\<lambda>s0. wait_out_cg ch2 ''a'' (\<lambda>s. val s X + 1) (\<lambda>d. init_single {''a'', ''b''})
+          (updg s0 ''a'' X 3))"
+  apply (rule spec_of_global_post)
+   apply (rule ex1') apply auto subgoal for s0
+    apply (rule entails_g_trans)
+     apply (rule sync_gassn_in_out) apply auto
+    apply (rule entails_g_trans)
+     apply (rule sync_gassn_subst_left) apply simp
+    apply (rule entails_g_trans)
+     apply (rule gassn_subst)
+    apply (rule entails_g_trans)
+     apply (rule sync_gassn_out_emp)
+      apply (auto simp add: ch1_def ch2_def)
+    apply (rule wait_out_cg_entails)
+    subgoal for d s0
+      apply (rule sync_gassn_emp) by auto
+    done
+  done
+
+subsubsection \<open>Example 2\<close>
+
+text \<open>
+   ch1!X; ch2?Y
+|| ch1?Z; ch2!(Z+1)
+\<close>
+
+definition ex2a :: "'a proc" where
+  "ex2a = (Cm (ch1[!](\<lambda>s. val s X)); Cm (ch2[?]Y))"
+
+lemma ex2a_sp:
+  "spec_of ex2a
+           (wait_out_c ch1 (\<lambda>s. val s X) (\<lambda>d. wait_in_c ch2 (\<lambda>d v. init {{Y := (\<lambda>_. v)}})))"
+  unfolding ex2a_def
+  apply (rule Valid_send_sp)
+  apply (rule spec_of_receive)
+  done
+
+definition ex2b :: "'a proc" where
+  "ex2b = (Cm (ch1[?]Z); Cm (ch2[!](\<lambda>s. val s Z + 1)))"
+
+lemma ex2b_sp:
+  "spec_of ex2b
+           (wait_in_c ch1 (\<lambda>d v. wait_out_c ch2 (\<lambda>s. val s Z + 1) (\<lambda>d. init) {{Z := (\<lambda>_. v)}}))"
+  unfolding ex2b_def
+  apply (rule Valid_receive_sp)
+  apply (rule spec_of_send)
+  done
+
+lemma ex2:
+  "spec_of_global
+    (Parallel (Single ''a'' ex2a)
+              {ch1, ch2}
+              (Single ''b'' ex2b))
+    (\<lambda>s0. init_single {''b'', ''a''}
+     (updg (updg s0 ''b'' Z (valg s0 ''a'' X)) ''a'' Y
+       (valg s0 ''a'' X + 1)))"
+proof -
+  have eq: "valg (updg s0 ''b'' Z (valg s0 ''a'' X)) ''b'' Z + 1 =
+        valg s0 ''a'' X + 1" for s0::"'a gstate"
+    by auto
+  show ?thesis
+  (* Stage 1: merge ex2_c and ex2_c' *)
+  apply (rule spec_of_global_post)
+   apply (rule spec_of_parallel)
+      apply (rule spec_of_single)
+      apply (rule ex2a_sp)
+  apply (rule spec_of_single)
+     apply (rule ex2b_sp)
+    apply simp apply simp
+  (* Stage 2: rewrite the assertions*)
+  apply auto subgoal for s0
+    apply (auto simp: single_assn_wait_in single_assn_wait_out updg_subst2 single_assn_init)
+  (* Stage 3: combine the two assertions *)
+    apply (rule entails_g_trans)
+     apply (rule sync_gassn_out_in) apply auto
+    apply (rule entails_g_trans)
+     apply (rule sync_gassn_subst_right) apply auto
+    apply (rule entails_g_trans)
+     apply (rule gassn_subst)
+    apply (rule entails_g_trans)
+     apply (rule sync_gassn_in_out) apply auto
+    apply (rule entails_g_trans)
+     apply (rule sync_gassn_subst_left) apply auto
+    apply (rule entails_g_trans)
+     apply (rule gassn_subst)
+    apply (rule entails_g_trans)
+       apply (rule sync_gassn_emp) apply simp
+      apply (simp only: valg_def[symmetric] eq)
+      by (rule entails_g_triv)
+    done
+qed
+
+subsubsection \<open>Example 3\<close>
+
+text \<open>
+   (ch1!A; B := B + 1)*
+|| (ch1?X; Y := Y + X)*
+\<close>
+definition ex3a :: "'a proc" where
+  "ex3a = (Rep (Cm (ch1[!](\<lambda>s. val s A)); B ::= (\<lambda>s. val s B + 1)))"
+
+fun rinv_c :: "nat \<Rightarrow> ('a estate \<Rightarrow> 'a assn) \<Rightarrow> ('a estate \<Rightarrow> 'a assn)" where
+  "rinv_c 0 Q = Q"
+| "rinv_c (Suc n) Q = wait_out_c ch1 (\<lambda>s. val s A) (\<lambda>d. rinv_c n Q {{ B := (\<lambda>s0. val s0 B + 1) }})"
+
+lemma ex3a_sp:
+  "spec_of ex3a
+           (\<lambda>s0. \<exists>\<^sub>an. rinv_c n init s0)"
+  unfolding ex3a_def
+  apply (rule spec_of_rep)
+  subgoal for n
+    apply (induction n)
+     apply simp apply (rule spec_of_skip)
+    subgoal premises pre for n
+      apply simp apply (rule spec_of_post)
+       apply (subst spec_of_seq_assoc)
+       apply (rule Valid_send_sp)
+       apply (rule Valid_assign_sp)
+       apply (rule pre) apply clarify
+      by (rule entails_triv)
+    done
+  done
+
+definition ex3b :: "'a proc" where
+  "ex3b = (Rep (Cm (ch1[?]X); Y ::= (\<lambda>s. val s Y + val s X)))"
+
+fun linv_c :: "nat \<Rightarrow> ('a estate \<Rightarrow> 'a assn) \<Rightarrow> ('a estate \<Rightarrow> 'a assn)" where
+  "linv_c 0 Q = Q"
+| "linv_c (Suc n) Q = wait_in_c ch1 (\<lambda>d v. linv_c n Q {{Y := (\<lambda>s. val s Y + val s X)}} {{X := (\<lambda>_. v)}} )"
+
+lemma ex3b_sp:
+  "spec_of ex3b
+           (\<lambda>s0. \<exists>\<^sub>an. linv_c n init s0)"
+  unfolding ex3b_def
+  apply (rule spec_of_rep)
+  subgoal for n
+    apply (induction n)
+     apply simp apply (rule spec_of_skip)
+    subgoal premises pre for n
+      apply simp apply (rule spec_of_post)
+       apply (subst spec_of_seq_assoc)
+       apply (rule Valid_receive_sp)
+       apply (rule Valid_assign_sp)
+       apply (rule pre) apply clarify
+      apply (rule entails_triv)
+      done
+    done
+  done
+
+definition ex3_inv :: "'a gstate \<Rightarrow> bool" where
+  "ex3_inv s0 \<longleftrightarrow> (valg s0 ''b'' Y = valg s0 ''a'' A * valg s0 ''a'' B)"
+
+lemma ex3':
+  assumes "ex3_inv s0"
+  shows
+  "\<exists>s1. ex3_inv s1 \<and>
+   (sync_gassn {ch1} {''a''} {''b''}
+     (single_assn ''a'' (rinv_c (Suc n1) init))
+     (single_assn ''b'' (linv_c (Suc n2) init)) s0 \<Longrightarrow>\<^sub>g
+    sync_gassn {ch1} {''a''} {''b''}
+     (single_assn ''a'' (rinv_c n1 init))
+     (single_assn ''b'' (linv_c n2 init)) s1)"
+proof -
+  have eq1: "updg (updg s0 ''b'' X (valg s0 ''a'' A)) ''a'' B
+              ((valg (updg s0 ''b'' X (valg s0 ''a'' A)) ''a'' B) + 1) =
+             updg (updg s0 ''b'' X (valg s0 ''a'' A)) ''a'' B (valg s0 ''a'' B + 1)"
+    by auto
+  let ?s1 = "updg (updg (updg s0 ''b'' X (valg s0 ''a'' A)) ''a'' B (valg s0 ''a'' B + 1)) ''b'' Y
+               (valg s0 ''b'' Y + valg s0 ''a'' A)"
+  show ?thesis
+  apply (rule exI[where x="?s1"])
+  apply (rule conjI)
+    subgoal using assms unfolding ex3_inv_def
+      apply (auto simp add: A_def B_def X_def Y_def)
+      by (auto simp add: algebra_simps)
+  subgoal
+    apply simp
+    apply (auto simp: single_assn_wait_in single_assn_wait_out updg_subst2)
+    apply (rule entails_g_trans)
+     apply (rule sync_gassn_out_in) apply auto
+    apply (rule entails_g_trans)
+     apply (rule sync_gassn_subst_right) apply auto
+    apply (rule entails_g_trans)
+     apply (rule gassn_subst)
+    apply (rule entails_g_trans)
+     apply (rule sync_gassn_subst_left) apply simp
+    apply (rule entails_g_trans)
+     apply (rule gassn_subst)
+    apply (simp only: valg_def[symmetric]) apply (subst eq1)
+    apply (rule entails_g_trans)
+     apply (rule sync_gassn_subst_right) apply auto
+    apply (rule entails_g_trans)
+     apply (rule gassn_subst)
+    apply (rule sync_gassn_triv)
+    apply (simp only: valg_def[symmetric])
+    by (auto simp add: X_def A_def B_def Y_def)
+  done
+qed
+
+lemma ex3'':
+  "ex3_inv s0 \<Longrightarrow>
+   \<exists>s1. ex3_inv s1 \<and>
+    (sync_gassn {ch1} {''a''} {''b''}
+      (single_assn ''a'' (rinv_c n1 init))
+      (single_assn ''b'' (linv_c n2 init)) s0 \<Longrightarrow>\<^sub>g
+    init_single {''b'', ''a''} s1)"
+proof (induction n1 n2 arbitrary: s0 rule: diff_induct)
+  case (1 n1)
+  show ?case
+  proof (cases n1)
+    case 0
+    show ?thesis
+      apply (subst 0)
+      apply (rule exI[where x=s0])
+      apply (rule conjI) using 1 apply simp
+      apply (rule entails_g_trans)
+      apply (auto simp add: single_assn_init)
+       apply (rule sync_gassn_emp) apply auto
+      by (rule entails_g_triv)
+  next
+    case (Suc n1)
+    show ?thesis
+      apply (subst Suc)
+      apply (rule exI[where x=s0])
+      apply (rule conjI) using 1 apply simp
+      apply auto
+       apply (auto simp add: single_assn_init single_assn_wait_out)
+       apply (rule sync_gassn_out_emp_unpair)
+      by auto
+  qed
+next
+  case (2 y)
+  show ?case
+    apply (rule exI[where x=s0])
+    apply (rule conjI) using 2 apply simp
+    apply auto
+    apply (auto simp add: single_assn_init single_assn_wait_in)
+    apply (rule sync_gassn_emp_in_unpair)
+    by auto
+next
+  case (3 n1 n2)
+  obtain s1 where s1: "ex3_inv s1"
+    "sync_gassn {ch1} {''a''} {''b''}
+      (single_assn ''a'' (rinv_c (Suc n1) init))
+      (single_assn ''b'' (linv_c (Suc n2) init)) s0 \<Longrightarrow>\<^sub>g
+     sync_gassn {ch1} {''a''} {''b''}
+      (single_assn ''a'' (rinv_c n1 init))
+      (single_assn ''b'' (linv_c n2 init)) s1"
+    using ex3' 3 by blast
+  obtain s2 where s2: "ex3_inv s2"
+    "sync_gassn {ch1} {''a''} {''b''} (single_assn ''a'' (rinv_c n1 init))
+       (single_assn ''b'' (linv_c n2 init)) s1 \<Longrightarrow>\<^sub>g
+     init_single {''b'', ''a''} s2"
+    using 3 s1(1) by blast 
+  show ?case
+    apply (rule exI[where x=s2])
+    apply (rule conjI) apply (rule s2)
+    apply (rule entails_g_trans)
+     apply (rule s1)
+    by (rule s2)
+qed
+
+lemma ex3''':
+  "spec_of_global
+    (Parallel (Single ''a'' ex3a)
+              {ch1}
+              (Single ''b'' ex3b))
+    (\<lambda>s0. \<exists>\<^sub>gn1 n2. sync_gassn {ch1} {''a''} {''b''}
+                    (single_assn ''a'' (rinv_c n1 init))
+                    (single_assn ''b'' (linv_c n2 init)) s0)"
+  (* Stage 1: merge ex3_c and ex4_c *)
+  apply (rule spec_of_global_post)
+   apply (rule spec_of_parallel)
+      apply (rule spec_of_single)
+  apply (rule ex3a_sp)
+     apply (rule spec_of_single)
+  apply (rule ex3b_sp) apply auto
+  apply (auto simp add: single_assn_exists sync_gassn_exists_left sync_gassn_exists_right)
+  by (rule entails_g_triv)
+
+lemma ex3:
+  "ex3_inv s0 \<Longrightarrow>
+    \<Turnstile>\<^sub>p {init_global s0}
+        (Parallel (Single ''a'' ex3a)
+                  {ch1}
+                  (Single ''b'' ex3b))
+       {\<exists>\<^sub>gs1. (\<lambda>s tr. ex3_inv s1 \<and> init_single {''b'', ''a''} s1 s tr)}"
+  apply (rule weaken_post_global[where R="\<exists>\<^sub>gn1 n2. sync_gassn {ch1} {''a''} {''b''}
+                    (single_assn ''a'' (rinv_c n1 init))
+                    (single_assn ''b'' (linv_c n2 init)) s0"])
+  subgoal by (auto simp: ex3'''[unfolded spec_of_global_def])
+  apply (auto simp add: exists_gassn_def entails_g_def)
+  subgoal for s tr n1 n2
+    using ex3''[of s0 n1 n2] unfolding entails_g_def
+    by auto
+  done
+
+subsubsection \<open>Example 5\<close>
+
+text \<open>
+  We analyze the following program for transmitting a list
+  to another process.
+
+  ( ch1!hd(ls); ls := tl ls )*
+    ||
+  ( ch1?X; ls := X # ls )*
+\<close>
+
+type_synonym ex5_state = "real list"
+
+definition ex5_left :: "ex5_state proc" where
+  "ex5_left = Rep (IF (\<lambda>s. epart s \<noteq> []) THEN
+                     (Cm (ch1[!](\<lambda>s. hd (epart s))); Basic (\<lambda>s. tl (epart s)))
+                   ELSE Skip FI)"
+
+fun ex5_linv_c :: "nat \<Rightarrow> ex5_state assn2 \<Rightarrow> ex5_state assn2" where
+  "ex5_linv_c 0 Q = Q"
+| "ex5_linv_c (Suc n) Q =
+   (IFA (\<lambda>s. epart s \<noteq> []) THEN
+      wait_out_c ch1 (\<lambda>s. hd (epart s)) (\<lambda>d. ex5_linv_c n Q {{ (\<lambda>s0. tl (epart s0)) }})
+    ELSE ex5_linv_c n Q FI)"
+
+lemma ex5_c:
+  "spec_of (RepN n (IF (\<lambda>s. epart s \<noteq> []) THEN
+                      (Cm (ch1[!](\<lambda>s. hd (epart s))); Basic (\<lambda>s. tl (epart s)))
+                    ELSE Skip FI))
+           (ex5_linv_c n init)"
+  apply (induction n)
+   apply simp apply (rule spec_of_skip)
+  subgoal premises pre for n
+    apply simp
+    apply (subst spec_of_cond_distrib)
+    apply (rule spec_of_cond)
+    subgoal
+      apply (rule spec_of_post)
+      apply (subst spec_of_seq_assoc)
+       apply (rule Valid_send_sp)
+       apply (rule Valid_basic_sp)
+      apply (rule pre) apply clarify
+      by (rule entails_triv)
+    subgoal
+      apply (rule spec_of_post)
+      apply (rule Valid_skip_sp)
+       apply (rule pre) apply clarify
+      by (rule entails_triv)
+    done
+  done
+
+definition ex5_right :: "ex5_state proc" where
+  "ex5_right = Rep (Cm (ch1[?]X); Basic (\<lambda>s. val s X # epart s))"
+
+fun ex5_rinv_c :: "nat \<Rightarrow> ex5_state assn2 \<Rightarrow> ex5_state assn2" where
+  "ex5_rinv_c 0 Q = Q"
+| "ex5_rinv_c (Suc n) Q =
+   wait_in_c ch1 (\<lambda>d v. ex5_rinv_c n Q {{ (\<lambda>s. val s X # epart s) }} {{ X := (\<lambda>_. v) }})"
+
+lemma ex5_c2:
+  "spec_of (RepN n (Cm (ch1[?]X); Basic (\<lambda>s. val s X # epart s)))
+           (ex5_rinv_c n init)"
+  apply (induction n)
+   apply simp apply (rule spec_of_skip)
+  subgoal premises pre for n
+    apply simp
+    apply (subst spec_of_seq_assoc)
+    apply (rule spec_of_post)
+     apply (rule Valid_receive_sp)
+     apply (rule Valid_basic_sp)
+     apply (rule pre) apply clarify
+    apply (rule entails_triv)      
+    done
+  done
+
+
+end
