lunarlander_sl/ext2/BigStepTask.thy
@@ -1,0 +1,21 @@
+theory BigStepTask
+  imports BigStepSimple
+begin
+
+subsection \<open>Start of testing for task\<close>
+
+type_synonym tid = real
+
+datatype status =
+  WAIT | READY | RUNNING
+
+datatype entered =
+  ezero | eone
+
+datatype task_st =
+  Sch (pool: "(real \<times> tid) list") (run_now: tid) (run_prior: real)
+| Task (status: status) (entered: entered) (task_prior: real)
+| None
+
+
+end
